src/util/basic.lean
@@ -1,4 +1,4 @@
-import data.pfun data.sigma data.zmod.basic
+import data.pfun data.sigma data.zmod.basic data.finmap
 
 namespace roption
 
@@ -63,6 +63,11 @@ inductive forall₂ {ι} {α α' : ι → Type*} (R : ∀ i, α i → α' i → 
   (Σ i, α i) → (Σ i, α' i) → Prop
 | mk (i a a') : R i a a' → forall₂ ⟨i, a⟩ ⟨i, a'⟩
 
+theorem forall₂.imp {ι} {α α' : ι → Type*}
+  {R S : ∀ i, α i → α' i → Prop} (H : ∀ i a a', R i a a' → S i a a') :
+  ∀ {s s'}, forall₂ R s s' → forall₂ S s s'
+| _ _ ⟨i, a, a', r⟩ := ⟨i, a, a', H _ _ _ r⟩
+
 theorem eta {α} {β : α → Type*} : ∀ x : Σ a, β a, (⟨x.1, x.2⟩ : Σ a, β a) = x
 | ⟨a, b⟩ := rfl
 
@@ -85,6 +90,14 @@ theorem update_at_forall₂' {α} {R : α → α → Prop} [is_refl α R]
   {n l₁ l₂} (h : update_at R n l₁ l₂) : forall₂ R l₁ l₂ :=
 (update_at_forall₂ h).imp (λ a b, or.rec id (by rintro rfl; apply refl))
 
+lemma forall₂_comm {α β} {r : α → β → Prop} {a b} :
+  forall₂ r a b ↔ forall₂ (flip r) b a := ⟨forall₂.flip, forall₂.flip⟩
+
+lemma forall₂_and_right {α β} {r : α → β → Prop} {p : β → Prop}
+  {l u} : forall₂ (λa b, r a b ∧ p b) l u ↔ forall₂ r l u ∧ (∀b∈u, p b) :=
+by rw [and_comm, forall₂_comm, @forall₂_comm _ _ r, ← forall₂_and_left];
+   conv in (_∧_) {rw and_comm}; refl
+
 lemma forall₂.mp_trans {α β γ} {r : α → β → Prop} {q : β → γ → Prop}
   {s : α → γ → Prop} (h : ∀a b c, r a b → q b c → s a c) :
   ∀{l₁ l₂ l₃}, forall₂ r l₁ l₂ → forall₂ q l₂ l₃ → forall₂ s l₁ l₃
@@ -97,7 +110,261 @@ lemma forall₂.nth {α β} {R : α → β → Prop} :
 | (a::l₁) (b::l₂) (forall₂.cons hr hrs) _  _  0     rfl rfl := hr
 | (a::l₁) (b::l₂) (forall₂.cons hr hrs) a' b' (n+1) h₁  h₂  := forall₂.nth hrs h₁ h₂
 
+lemma map_prod_fst_eq_of_forall₂_eq {α β γ} {R : β → γ → Prop} {l₁ l₂}
+  (h : forall₂ (prod.forall₂ (@eq α) R) l₁ l₂) :
+  l₁.map prod.fst = l₂.map prod.fst :=
+begin
+  rw [← list.forall₂_eq_eq_eq, list.forall₂_map_left_iff,
+    list.forall₂_map_right_iff],
+  refine h.imp _, rintro _ _ ⟨rfl, _⟩, refl
+end
+
+lemma map_sigma_fst_eq_of_forall₂_eq {α} {β β' : α → Type*}
+  {R : ∀ a, β a → β' a → Prop} {l₁ l₂}
+  (h : forall₂ (sigma.forall₂ R) l₁ l₂) :
+  l₁.map sigma.fst = l₂.map sigma.fst :=
+begin
+  rw [← list.forall₂_eq_eq_eq, list.forall₂_map_left_iff,
+    list.forall₂_map_right_iff],
+  refine h.imp _, rintro _ _ ⟨⟩, refl
+end
+
+lemma rel_of_forall₂_of_nodup {α β γ} {R : β → γ → Prop} {l₁ l₂}
+  (h : forall₂ (prod.forall₂ (@eq α) R) l₁ l₂)
+  (nd : (l₁.map prod.fst).nodup)
+  {a b c} (h₁ : (a, b) ∈ l₁) (h₂ : (a, c) ∈ l₂) : R b c :=
+begin
+  have nd' := nd, rw map_prod_fst_eq_of_forall₂_eq h at nd',
+  induction h, {cases h₁},
+  rcases h₁ with rfl | h₁; rcases h₂ with rfl | h₂,
+  { cases h_a_1, assumption },
+  { rcases h_a_1 with ⟨i, _, _, τ', rfl, _⟩,
+    cases (list.nodup_cons.1 nd').1 (list.mem_map_of_mem prod.fst h₂:_) },
+  { rcases h_a_1 with ⟨i, v', _, _, rfl, _⟩,
+    cases (list.nodup_cons.1 nd).1 (list.mem_map_of_mem prod.fst h₁:_) },
+  { exact h_ih (list.nodup_cons.1 nd).2 h₁ h₂ (list.nodup_cons.1 nd').2 }
+end
+
+theorem lookmap_forall₂ {α} (f : α → option α) :
+  ∀ l, forall₂ (λ a b, a = b ∨ b ∈ f a) l (lookmap f l)
+| []     := forall₂.nil
+| (a::l) := begin
+  dsimp only [lookmap],
+  cases e : f a,
+  { exact forall₂.cons (or.inl rfl) (lookmap_forall₂ l) },
+  { refine forall₂.cons (or.inr e) (@forall₂_refl _ _ ⟨_⟩ l),
+    exact λ _, or.inl rfl },
+end
+
+theorem lookmap_forall₂' {α} (f : α → option α)
+  {β} (g : α → β) (H : ∀ a a' (b ∈ f a) (b' ∈ f a'), g a = g a') :
+  ∀ l : list α, (l.map g).nodup → forall₂ (λ a b, (f a).get_or_else a = b) l (lookmap f l)
+| []     nd := forall₂.nil
+| (a::l) nd := begin
+  cases list.nodup_cons.1 nd with nd₁ nd₂,
+  dsimp only [lookmap],
+  cases e : f a,
+  { exact forall₂.cons (by rw e; refl) (lookmap_forall₂' l nd₂) },
+  { refine forall₂.cons (by rw e; refl) (forall₂_same $ λ a' h, _),
+    cases e' : f a', {refl},
+    rw H _ _ _ e _ e' at nd₁,
+    cases nd₁ (mem_map_of_mem _ h) },
+end
+
+inductive kreplace_rel {α} {β : α → Type*} (a) (b : β a) : ∀ a, β a → β a → Prop
+| repl {} {b'} : kreplace_rel a b' b
+| refl {} {a' b'} : a ≠ a' → kreplace_rel a' b' b'
+
+theorem kreplace_forall₂ {α} {β : α → Type*} [decidable_eq α] (a) (b : β a)
+  {l} (nd : nodupkeys l) : forall₂ (sigma.forall₂ (kreplace_rel a b)) l (kreplace a b l) :=
+begin
+  refine (lookmap_forall₂' _ _ _ _ nd).imp _,
+  { rintro ⟨a₁, b₁⟩ ⟨a₂, b₂⟩ h,
+    split_ifs at h; cases h,
+    { cases h_1, exact ⟨_, _, _, kreplace_rel.repl⟩ },
+    { exact ⟨_, _, _, kreplace_rel.refl h_1⟩ } },
+  { rintro ⟨a₁, b₁⟩ ⟨a₂, b₂⟩ s₁ h₁ s₂ h₂,
+    split_ifs at h₁ h₂; cases h₁; cases h₂,
+    exact h_1.symm.trans h }
+end
+
+theorem mem_erasep {α} (p : α → Prop) [decidable_pred p] {l : list α}
+  (H : pairwise (λ a b, p a → p b → false) l)
+  {a : α} : a ∈ erasep p l ↔ ¬ p a ∧ a ∈ l :=
+⟨λ h, begin
+  by_cases pa : p a,
+  { rcases exists_of_erasep (mem_of_mem_erasep h) pa
+      with ⟨b, l₁, l₂, h₁, pb, rfl, h₂⟩,
+    rw h₂ at h,
+    cases mem_append.1 h,
+    { cases h₁ _ h_1 pa },
+    { cases (pairwise_cons.1 (pairwise_append.1 H).2.1).1 _ h_1 pb pa } },
+  { exact ⟨pa, (mem_erasep_of_neg pa).1 h⟩ }
+end, λ ⟨h₁, h₂⟩, (mem_erasep_of_neg h₁).2 h₂⟩
+
+theorem mem_kerase {α β} [decidable_eq α] {s : list (sigma β)}
+  (nd : s.nodupkeys) {a a' : α} {b' : β a'} :
+  sigma.mk a' b' ∈ kerase a s ↔ a ≠ a' ∧ sigma.mk a' b' ∈ s :=
+mem_erasep _ $ (nodupkeys_iff_pairwise.1 nd).imp $
+by rintro x y h rfl; exact h
+
 end list
+
+def prod.to_sigma {α β} (x : α × β) : Σ a : α, β := ⟨x.1, x.2⟩
+
+namespace alist
+open list
+
+theorem mem_lookup_iff {α} {β : α → Type*} [decidable_eq α]
+  {a : α} {b : β a} {s : alist α β} :
+  b ∈ lookup a s ↔ sigma.mk a b ∈ s.entries :=
+list.mem_lookup_iff s.2
+
+theorem exists_mem_lookup_iff {α} {β : α → Type*} [decidable_eq α]
+  {a : α} {s : alist α β} : (∃ b, b ∈ lookup a s) ↔ a ∈ s :=
+option.is_some_iff_exists.symm.trans lookup_is_some
+
+theorem to_sigma_nodupkeys {α β} {l : list (α × β)} :
+  (l.map prod.to_sigma).nodupkeys ↔ (l.map prod.fst).nodup :=
+by rw [list.nodupkeys, list.map_map]; refl
+
+def mk' {α β} (l : list (α × β)) (h : (l.map prod.fst).nodup) : alist α (λ _, β) :=
+⟨l.map prod.to_sigma, to_sigma_nodupkeys.2 h⟩
+
+@[simp] theorem mk'_entries {α β} (l : list (α × β)) (h) :
+  (mk' l h).entries = l.map prod.to_sigma := rfl
+
+@[simp] theorem mk'_keys {α β} (l : list (α × β)) (h) :
+  (mk' l h).keys = l.map prod.fst :=
+by rw [keys, mk'_entries, list.map_map]; refl
+
+def cons {α} {β : α → Type*} (s : alist α β)
+  (a : α) (b : β a) (h : a ∉ s) : alist α β :=
+⟨⟨a, b⟩ :: s.entries, nodup_cons.2 ⟨mt mem_keys.1 h, s.nodupkeys⟩⟩
+
+theorem insert_eq_cons {α} {β : α → Type*} [decidable_eq α]
+  {s : alist α β} {a : α} {b : β a} (h : a ∉ s) : insert a b s = cons s a b h :=
+dif_neg h
+
+theorem lookup_cons_of_lookup {α β} [decidable_eq α] {s a b h a' b'}
+  (H : b' ∈ lookup a' s) : b' ∈ lookup a' (@cons α β s a b h) :=
+mem_lookup_iff.2 $ or.inr $ mem_lookup_iff.1 H
+
+theorem lookup_cons_self {α β} [decidable_eq α] {s a b h} :
+  b ∈ lookup a (@cons α β s a b h) :=
+mem_lookup_iff.2 $ or.inl rfl
+
+def forall₂ {α} {β γ : α → Type*} (R : ∀ a, β a → γ a → Prop)
+  (l₁ : alist α β) (l₂ : alist α γ) : Prop :=
+list.forall₂ (sigma.forall₂ R) l₁.entries l₂.entries
+
+theorem forall₂.imp {α} {β β' : α → Type*}
+  {R S : ∀ a, β a → β' a → Prop} (H : ∀ a b b', R a b b' → S a b b')
+  {s s'} : forall₂ R s s' → forall₂ S s s' :=
+list.forall₂.imp $ λ a b, sigma.forall₂.imp H
+
+theorem forall₂.keys {α} {β β' : α → Type*}
+  {R : ∀ a, β a → β' a → Prop} {s s'} :
+  forall₂ R s s' → s.keys = s'.keys :=
+map_sigma_fst_eq_of_forall₂_eq
+
+theorem forall₂.mem_iff {α} {β β' : α → Type*}
+  {R : ∀ a, β a → β' a → Prop} {s s'} (H : forall₂ R s s')
+  {a} : a ∈ s ↔ a ∈ s' :=
+by rw [← mem_keys, H.keys, mem_keys]
+
+theorem forall₂.rel_of_mem {α} {β₁ β₂ : α → Type*} [decidable_eq α]
+  {R : ∀ a, β₁ a → β₂ a → Prop} {s₁ s₂} (H : forall₂ R s₁ s₂)
+  {a} {b₁ : β₁ a} {b₂ : β₂ a}
+  (h₁ : sigma.mk a b₁ ∈ s₁.entries)
+  (h₂ : sigma.mk a b₂ ∈ s₂.entries) : R a b₁ b₂ :=
+begin
+  cases s₁ with l₁ nd₁, cases s₂ with l₂ nd₂,
+  dsimp only [forall₂] at *,
+  induction H, {cases h₁},
+  rcases h₁ with rfl | h₁; rcases h₂ with rfl | h₂,
+  { cases H_a_1, assumption },
+  { rcases H_a_1 with ⟨i, _, b₂', _⟩,
+    cases (list.nodupkeys_cons.1 nd₂).1 _ h₂ },
+  { rcases H_a_1 with ⟨i, b₁', _, _⟩,
+    cases (list.nodupkeys_cons.1 nd₁).1 _ h₁ },
+  { cases H_a, cases H_b,
+    exact H_ih (list.nodupkeys_cons.1 nd₁).2 h₁ (list.nodupkeys_cons.1 nd₂).2 h₂ }
+end
+
+theorem forall₂.rel_of_lookup {α} {β β' : α → Type*} [decidable_eq α]
+  {R : ∀ a, β a → β' a → Prop} {s s'} (H : forall₂ R s s')
+  {a b b'} (h₁ : b ∈ s.lookup a) (h₂ : b' ∈ s'.lookup a) : R a b b' :=
+by rw mem_lookup_iff at h₁ h₂; exact H.rel_of_mem h₁ h₂
+
+theorem forall₂.rel_of_lookup_right {α} {β β' : α → Type*} [decidable_eq α]
+  {R : ∀ a, β a → β' a → Prop} {s s'} (H : forall₂ R s s')
+  {a b} (h : b ∈ s.lookup a) : ∃ b' ∈ s'.lookup a, R a b b' :=
+let ⟨b', h'⟩ := exists_mem_lookup_iff.2
+  (H.mem_iff.1 (exists_mem_lookup_iff.1 ⟨_, h⟩)) in
+⟨b', h', H.rel_of_lookup h h'⟩
+
+theorem replace_forall₂ {α} {β : α → Type*} [decidable_eq α]
+  (a) (b : β a) (s : alist α β) : forall₂ (kreplace_rel a b) s (replace a b s) :=
+kreplace_forall₂ _ _ s.2
+
+@[simp] theorem entries_erase {α β} [decidable_eq α] (a : α) (s : alist α β) :
+  (erase a s).entries = s.entries.kerase a := rfl
+
+theorem lookup_erase {α β} [decidable_eq α] {s : alist α β} {a a' : α} {b' : β a'} :
+  b' ∈ lookup a' (erase a s) ↔ a ≠ a' ∧ b' ∈ lookup a' s :=
+by rw [mem_lookup_iff, entries_erase, mem_kerase s.2, mem_lookup_iff]
+
+def values {α β} (s : alist α (λ _, β)) : list β := s.entries.map sigma.snd
+
+@[elab_as_eliminator]
+def rec' {α β} {C : alist α β → Sort*}
+  (H0 : C ∅) (H1 : ∀ s a b h, C s → C (cons s a b h)) (s) : C s :=
+begin
+  cases s with l nd,
+  induction l with ab l IH,
+  { exact H0 },
+  { cases ab with a b,
+    have := list.nodupkeys_cons.1 nd,
+    exact H1 ⟨l, this.2⟩ a b (not_exists.2 this.1) (IH this.2) }
+end
+
+@[simp] theorem rec'_empty {α β C H0 H1} : @rec' α β C H0 H1 ∅ = H0 := rfl
+
+@[simp] theorem rec'_cons {α β C H0 H1} : ∀ s a b h,
+  @rec' α β C H0 H1 (cons s a b h) = H1 s a b h (@rec' α β C H0 H1 s)
+| ⟨l, nd⟩ a b h := rfl
+
+end alist
+
+namespace finmap
+open list
+
+theorem mem_lookup_iff {α} {β : α → Type*} [decidable_eq α]
+  {a : α} {b : β a} {s : finmap α β} :
+  b ∈ lookup a s ↔ sigma.mk a b ∈ s.entries :=
+induction_on s $ λ s, alist.mem_lookup_iff
+
+theorem exists_mem_lookup_iff {α} {β : α → Type*} [decidable_eq α]
+  {a : α} {s : finmap α β} : (∃ b, b ∈ lookup a s) ↔ a ∈ s :=
+induction_on s $ λ s, alist.exists_mem_lookup_iff
+
+theorem lookup_insert_of_neg {α} {β : α → Type*} [decidable_eq α]
+  {a : α} {b : β a} {s : finmap α β} (h : a ∉ s) {a' : α} {b' : β a'} :
+  b' ∈ (insert a b s).lookup a' ↔
+  sigma.mk a' b' = ⟨a, b⟩ ∨ b' ∈ s.lookup a' :=
+by rw [mem_lookup_iff, mem_lookup_iff, insert_entries_of_neg h, multiset.mem_cons]
+
+theorem lookup_insert_self {α β} [decidable_eq α] {s a b} :
+  a ∉ s → b ∈ lookup a (@insert α β _ a b s) :=
+induction_on s $ λ s h,
+by simp [insert, alist.insert_eq_cons h]; exact alist.lookup_cons_self
+
+theorem lookup_erase {α β} [decidable_eq α] {s : finmap α β} {a a' : α} {b' : β a'} :
+  b' ∈ lookup a' (erase a s) ↔ a ≠ a' ∧ b' ∈ lookup a' s :=
+induction_on s $ λ s, alist.lookup_erase
+
+end finmap
 
 def int32 := zmod (2^32)
 
